if-cubic-invalid.c        & $(\textsf{EF}(p=0)) \wedge (\textsf{EF}(p=1))$ \\
if-cubic-valid.c          & $(\textsf{EF}(p=0)) \wedge (\textsf{EF}(p=1))$ \\
if-nla-invalid.c          & $(\textsf{EF}(p=0)) \wedge (\textsf{EF}(p=1))$ \\
if-nla-valid.c            & $(\textsf{EF}(p=0)) \wedge (\textsf{EF}(p=1))$ \\
square-loop-nla-invalid.c & $(\textsf{EF}(p=0)) \wedge (\textsf{EF}(p=1))$ \\
square-loop-nla-valid.c   & $(\textsf{EF}(p=0)) \wedge (\textsf{EF}(p=1))$ \\
while-cubic-invalid.c     & $(\textsf{EF}(p=0)) \wedge (\textsf{EF}(p=1))$ \\
while-cubic-valid.c       & $(\textsf{EF}(p=0)) \wedge (\textsf{EF}(p=1))$ \\
while-nla-invalid.c       & $(\textsf{EF}(p=0)) \wedge (\textsf{EF}(p=1))$ \\
while-nla-valid.c         & $(\textsf{EF}(p=0)) \wedge (\textsf{EF}(p=1))$ \\
