\ttt{neg-afagp-F.c} & \rExact  & 289.7    & 2  & D, USC, V, ExtN, V, V & $\ell_{18}:((((((z   z) - (12   y)) - (6   z)) + 12) + c) <= k)$ $\mapsto$ $0 \geq c-k,k-c \leq -1$  \\
\ttt{neg-afagp-T.c} & \rExact  & 294.7    & 2  & D, USC, V, ExtN, V, V & $\ell_{18}:((((((z   z) - (12   y)) - (6   z)) + 12) + c) <= k)$ $\mapsto$ $0 \geq c-k,k-c \leq -1$  \\
\ttt{neg-afefp-F.c} & \rExact  & 229.4    & 2  & D, USC, V, ExtN, V, V & $\ell_{18}:((((((z   z) - (12   y)) - (6   z)) + 12) + c) <= k)$ $\mapsto$ $(0 >= (-(k) + n)),(((0 + (n   -1)) + (k   1)) <= -1)$  \\
\ttt{neg-afegp-F.c} & \rExact  & 227.6    & 2  & D, USC, V, ExtN, V, V & $\ell_{18}:((((((z   z) - (12   y)) - (6   z)) + 12) + c) <= k)$ $\mapsto$ $0 \geq c-k,k-c \leq -1$  \\
\ttt{neg-afegp-T.c} & \rExact  & 223.7    & 2  & D, USC, V, ExtN, V, V & $\ell_{18}:((((((z   z) - (12   y)) - (6   z)) + 12) + c) <= k)$ $\mapsto$ $0 \geq c-k,k-c \leq -1$  \\
\ttt{neg-afp-F.c} & \rExact  & 164.2    & 2  & D, USC, V, ExtN, V, V & $\ell_{18}:((((((z   z) - (12   y)) - (6   z)) + 12) + c) <= k)$ $\mapsto$ $(0 >= (-(k) + n)),(((0 + (k   1)) + (n   -1)) <= -1)$  \\
\ttt{neg-afp-T.c} & \rExact  & 165.6    & 2  & D, USC, V, ExtN, V, V & $\ell_{18}:((((((z   z) - (12   y)) - (6   z)) + 12) + c) <= k)$ $\mapsto$ $0 \geq c-k,k-c \leq -1$  \\
\ttt{neg-efafp-F.c} & \rExact  & 244.7    & 2  & D, USC, V, ExtN, V, V & $\ell_{31}:((((((z   z) - (12   y)) - (6   z)) + 12) + c) <= k)$ $\mapsto$ $(0 >= (-(k) + n)),(((0 + (k   1)) + (n   -1)) <= -1)$  \\
\ttt{neg-egafp-F.c} & \rExact  & 282.8    & 2  & D, USC, V, ExtN, V, V & $\ell_{19}:((((((z   z) - (12   y)) - (6   z)) + 12) + c) <= k)$ $\mapsto$ $0 \geq c-k,k-c \leq -1$  \\
\ttt{neg-egafp-T.c} & \rExact  & 290.6    & 2  & D, USC, V, ExtN, V, V & $\ell_{19}:((((((z   z) - (12   y)) - (6   z)) + 12) + c) <= k)$ $\mapsto$ $0 \geq c-k,k-c \leq -1$  \\
\ttt{neg-egimpafp-T.c} & \rExact  & 215.5    & 2  & D, USC, V, ExtN, V, V & $\ell_{20}:((((((z   z) - (12   y)) - (6   z)) + 12) + c) <= k)$ $\mapsto$ $(0 >= (-(k) + n)),(((0 + (k   1)) + (n   -1)) <= -1)$  \\
