\ttt{if-cubic-F.c} & \rExact  & 51.5     & 3  & v,tn,v,en,v,v & $\ell_{6}:(8 == ((x   x)   x))$ $\mapsto$ $(((4 >= (p + x)) \&\& (0 >= (p - x)) \&\& (0 >= (-(p) + x)) \&\& ((-(p) - x) <= -(4))) || ((2 >= p) \&\& (0 >= (-(p) + x)) \&\& ((-(p) - x) <= -(4)))),(((0 == (p - 2)) \&\& (1 >= (p - x)) \&\& !(((2 >= p) \&\& (0 >= (-(p) + x)) \&\& ((-(p) - x) <= -(4))))) || (0 >= x))$  \\
\ttt{if-cubic-T.c} & \rExact  & 51.3     & 3  & v,tn,v,en,v,v & $\ell_{6}:(8 == ((x   x)   x))$ $\mapsto$ $(((2 >= p) \&\& (0 >= (-(p) + x)) \&\& ((-(p) - x) <= -(4))) || ((-(x) <= -(2)) \&\& (4 >= (p + x)) \&\& (0 >= (-(p) + x)))),(((0 == (p - 2)) \&\& (0 >= -(x)) \&\& !(((-(x) <= -(2)) \&\& (4 >= (p + x)) \&\& (0 >= (-(p) + x))))) || (1 >= (p + x)))$  \\
\ttt{if-F.c}    & \rExact  & 78.8     & 6  & v,tn,v,ep,v,tp,v,tn,v,tp,v,v & $\ell_{6}:(36 == (x   x))$ $\mapsto$ $((((0 + (x   1)) <= 6) \&\& !(((0 == (p - 2)) \&\& ((-(p) + x) <= -(1))))) || ((x <= -(6)) \&\& (-(p) <= -(2)) \&\& (8 >= (p - x))))\&\&!(((0 == (p - 2)) \&\& (0 >= (p - x)) \&\& (3 >= (-(p) + x)))),(((((0 == (p - 2)) \&\& (0 >= -(x)) \&\& !(((2 >= p) \&\& (-(x) <= -(6)) \&\& (4 >= (-(p) + x))))) || ((0 == (p - 2)) \&\& ((-(p) + x) <= -(1)))) \&\& !(((x <= -(6)) \&\& (-(p) <= -(2)) \&\& (8 >= (p - x))))) || ((0 == (p - 2)) \&\& (0 >= (p - x)) \&\& (3 >= (-(p) + x))))$  \\
\ttt{if-T.c}    & \rExact  & 76.5     & 6  & v,tn,v,ep,v,tp,v,tn,v,tp,v,v & $\ell_{7}:(36 == (x   x))$ $\mapsto$ $(((((0 + (x   1)) + (p   1)) <= 8) \&\& !(((0 == (p - 2)) \&\& (3 >= x)))) || ((-(p) <= -(2)) \&\& (8 >= (p - x)) \&\& ((p + x) <= -(4))))\&\&!(((2 >= p) \&\& (5 >= x) \&\& (-(p) <= -(2)) \&\& ((-(p) - x) <= -(6)))),(((((0 == (p - 2)) \&\& (1 >= (p - x)) \&\& !(((6 >= x) \&\& (-(p) <= -(2)) \&\& ((p - x) <= -(4))))) || ((0 == (p - 2)) \&\& (3 >= x))) \&\& !(((-(p) <= -(2)) \&\& (8 >= (p - x)) \&\& ((p + x) <= -(4))))) || ((2 >= p) \&\& (5 >= x) \&\& (-(p) <= -(2)) \&\& ((-(p) - x) <= -(6))))$  \\
\ttt{square-loop-F.c} & \rExact  & 383.6    & 12 & v,tn,v,tn,v,tn,v,tn,v,tn,v,tn,v,tn,v,tn,v,tn,v,tn,v,tn,v,v & $\ell_{8}:(49 < (x   x))$ $\mapsto$ $((((((((((((-(x) <= -(8)) || ((0 == (p - 2)) \&\& (3 >= y) \&\& ((-(p) - y) <= -(3)) \&\& ((-(p) + x) <= -(10)))) || ((0 == (p - 2)) \&\& (7 >= (p + y)) \&\& ((x + y) <= -(4)) \&\& ((-(p) - y) <= -(6)))) || ((0 == (p - 2)) \&\& (10 >= y) \&\& ((-(p) - y) <= -(7)) \&\& ((-(p) + x) <= -(10)))) || ((0 == (p - 2)) \&\& (x <= -(8)) \&\& (10 >= (-(p) + y)) \&\& ((-(p) - y) <= -(13)))) || ((0 == (p - 2)) \&\& (x <= -(8)) \&\& (16 >= (-(p) + y)) \&\& ((-(p) - y) <= -(15)))) || ((0 == (p - 2)) \&\& ((p + x) <= -(6)) \&\& ((p - y) <= -(17)) \&\& (19 >= (-(p) + y)))) || ((0 == (p - 2)) \&\& (17 >= (x + y)) \&\& ((p - y) <= -(20)) \&\& ((-(p) + x) <= -(10)))) || ((0 == (p - 2)) \&\& ((p + x) <= -(6)) \&\& ((-(x) - y) <= -(18)))) || ((0 == (p - 1)) \&\& (14 >= y) \&\& (5 >= (x + y)) \&\& (0 >= (p - y)) \&\& ((-(p) + x) <= -(9)))) || ((0 == (p - 1)) \&\& (8 >= (x + y)) \&\& ((p - y) <= -(13)) \&\& ((-(p) + x) <= -(9)))) || ((0 == (p - 1)) \&\& ((-(x) - y) <= -(9)) \&\& ((-(p) + x) <= -(9)))),(7 >= x)\&\&!(((0 == (p - 2)) \&\& (3 >= y) \&\& ((-(p) - y) <= -(3)) \&\& ((-(p) + x) <= -(10))))\&\&!(((0 == (p - 2)) \&\& (7 >= (p + y)) \&\& ((x + y) <= -(4)) \&\& ((-(p) - y) <= -(6))))\&\&!(((0 == (p - 2)) \&\& (10 >= y) \&\& ((-(p) - y) <= -(7)) \&\& ((-(p) + x) <= -(10))))\&\&!(((0 == (p - 2)) \&\& (x <= -(8)) \&\& (10 >= (-(p) + y)) \&\& ((-(p) - y) <= -(13))))\&\&!(((0 == (p - 2)) \&\& (x <= -(8)) \&\& (16 >= (-(p) + y)) \&\& ((-(p) - y) <= -(15))))\&\&!(((0 == (p - 2)) \&\& ((p + x) <= -(6)) \&\& ((p - y) <= -(17)) \&\& (19 >= (-(p) + y))))\&\&!(((0 == (p - 2)) \&\& (17 >= (x + y)) \&\& ((p - y) <= -(20)) \&\& ((-(p) + x) <= -(10))))\&\&!(((0 == (p - 2)) \&\& ((p + x) <= -(6)) \&\& ((-(x) - y) <= -(18))))\&\&!(((0 == (p - 1)) \&\& (14 >= y) \&\& (5 >= (x + y)) \&\& (0 >= (p - y)) \&\& ((-(p) + x) <= -(9))))\&\&!(((0 == (p - 1)) \&\& (8 >= (x + y)) \&\& ((p - y) <= -(13)) \&\& ((-(p) + x) <= -(9))))\&\&!(((0 == (p - 1)) \&\& ((-(x) - y) <= -(9)) \&\& ((-(p) + x) <= -(9))))$  \\
\ttt{square-loop-T.c} & \rExact  & 233.3    & 7  & v,tn,v,tn,v,tn,v,tn,v,tn,v,tn,v,v & $\ell_{8}:(49 < (x   x))$ $\mapsto$ $(((((((-(x) <= -(8)) || ((0 == (p - 2)) \&\& (1 >= (p - y)) \&\& (5 >= (p + y)) \&\& ((p + x) <= -(6)))) || ((0 == (p - 2)) \&\& (5 >= y) \&\& (-(y) <= -(4)) \&\& ((x + y) <= -(4)))) || ((0 == (p - 2)) \&\& ((p + x) <= -(6)) \&\& ((x + y) <= -(1)) \&\& ((-(p) - y) <= -(7)))) || ((0 == (p - 2)) \&\& (0 >= (-(x) - y)) \&\& ((-(p) + x) <= -(10)))) || ((0 == (p - 1)) \&\& (0 >= (p - y)) \&\& ((x + y) <= -(6)) \&\& ((-(p) + x) <= -(9)))) || ((0 == (p - 1)) \&\& (x <= -(8)) \&\& (5 >= (-(x) - y)))),(7 >= x)\&\&!(((0 == (p - 2)) \&\& (1 >= (p - y)) \&\& (5 >= (p + y)) \&\& ((p + x) <= -(6))))\&\&!(((0 == (p - 2)) \&\& (5 >= y) \&\& (-(y) <= -(4)) \&\& ((x + y) <= -(4))))\&\&!(((0 == (p - 2)) \&\& ((p + x) <= -(6)) \&\& ((x + y) <= -(1)) \&\& ((-(p) - y) <= -(7))))\&\&!(((0 == (p - 2)) \&\& (0 >= (-(x) - y)) \&\& ((-(p) + x) <= -(10))))\&\&!(((0 == (p - 1)) \&\& (0 >= (p - y)) \&\& ((x + y) <= -(6)) \&\& ((-(p) + x) <= -(9))))\&\&!(((0 == (p - 1)) \&\& (x <= -(8)) \&\& (5 >= (-(x) - y))))$  \\
\ttt{while-cubic-F.c} & \rExact  & 87.0     & 7  & v,tn,v,ep,v,tp,v,tn,v,tp,v,tn,v,v & $\ell_{6}:((64 >= ((y   y)   y)) \&\& (1 <= (y   y)))$ $\mapsto$ $(((((((0 + (p   1)) + (y   1)) <= 6) \&\& !(((0 >= y) \&\& (2 >= (p - y)) \&\& ((-(p) - y) <= -(2))))) || ((0 == (p - 1)) \&\& (5 >= (p + y)) \&\& ((p - y) <= -(1)))) \&\& !(((1 >= p) \&\& (0 >= -(y)) \&\& (-(p) <= -(1)) \&\& (4 >= (-(p) + y))))) || ((0 == (p - 1)) \&\& (4 >= y) \&\& ((p - y) <= -(1)))),(((((-(p) <= -(1)) \&\& (0 >= -(y)) \&\& ((-(p) - y) <= -(2)) \&\& !(((0 == (p - 2)) \&\& (4 >= y) \&\& ((-(p) - y) <= -(3))))) || ((0 >= y) \&\& (2 >= (p - y)) \&\& ((-(p) - y) <= -(2)))) \&\& !(((0 == (p - 1)) \&\& (5 >= (p + y)) \&\& ((p - y) <= -(1))))) || ((1 >= p) \&\& (0 >= -(y)) \&\& (-(p) <= -(1)) \&\& (4 >= (-(p) + y))))\&\&!(((0 == (p - 1)) \&\& (4 >= y) \&\& ((p - y) <= -(1))))$  \\
\ttt{while-cubic-T.c} & \rExact  & 84.4     & 7  & v,tn,v,ep,v,tp,v,tn,v,tp,v,tn,v,v & $\ell_{6}:((64 >= ((y   y)   y)) \&\& (1 <= (y   y)))$ $\mapsto$ $(((((((0 + (p   1)) + (y   1)) <= 6) \&\& !(((0 >= -(y)) \&\& (-(p) <= -(2)) \&\& (2 >= (p + y))))) || ((0 == (p - 1)) \&\& (4 >= y) \&\& (-(y) <= -(2)))) \&\& !(((1 >= p) \&\& (5 >= y) \&\& (0 >= -(y)) \&\& (-(p) <= -(1))))) || ((0 == (p - 1)) \&\& ((p - y) <= -(1)) \&\& (3 >= (-(p) + y)))),(((((0 >= -(y)) \&\& ((-(p) - y) <= -(2)) \&\& !(((0 == (p - 2)) \&\& (4 >= y) \&\& (-(y) <= -(1))))) || ((0 >= -(y)) \&\& (-(p) <= -(2)) \&\& (2 >= (p + y)))) \&\& !(((0 == (p - 1)) \&\& (4 >= y) \&\& (-(y) <= -(2))))) || ((1 >= p) \&\& (5 >= y) \&\& (0 >= -(y)) \&\& (-(p) <= -(1))))\&\&!(((0 == (p - 1)) \&\& ((p - y) <= -(1)) \&\& (3 >= (-(p) + y))))$  \\
\ttt{while-F.c} & \rExact  & 190.4    & 6  & v,tn,v,tn,v,tn,v,tn,v,tn,v,v & $\ell_{9}:(63 <= ((x   x) - (2   x)))$ $\mapsto$ $((((((((p - x) <= -(7)) \&\& ((-(p) - x) <= -(10))) || ((0 == (p - 2)) \&\& (1 >= (p - y)) \&\& (0 >= (-(p) + y)) \&\& ((x + y) <= -(6)))) || ((0 == (p - 2)) \&\& (0 >= (p - y)) \&\& ((x + y) <= -(5)))) || ((0 == (p - 2)) \&\& (4 >= (-(x) - y)) \&\& ((-(p) + x) <= -(9)))) || ((0 == (p - 1)) \&\& (4 >= (p + y)) \&\& (0 >= (p - y)) \&\& ((x + y) <= -(8)))) || ((0 == (p - 1)) \&\& (0 >= (p - y)) \&\& ((-(p) + x) <= -(8)))),(8 >= x)\&\&!(((0 == (p - 2)) \&\& (1 >= (p - y)) \&\& (0 >= (-(p) + y)) \&\& ((x + y) <= -(6))))\&\&!(((0 == (p - 2)) \&\& (0 >= (p - y)) \&\& ((x + y) <= -(5))))\&\&!(((0 == (p - 2)) \&\& (4 >= (-(x) - y)) \&\& ((-(p) + x) <= -(9))))\&\&!(((0 == (p - 1)) \&\& (4 >= (p + y)) \&\& (0 >= (p - y)) \&\& ((x + y) <= -(8))))\&\&!(((0 == (p - 1)) \&\& (0 >= (p - y)) \&\& ((-(p) + x) <= -(8))))$  \\
\ttt{while-T.c} & \rExact  & 189.6    & 6  & v,tn,v,tn,v,tn,v,tn,v,tn,v,v & $\ell_{9}:(63 <= ((x   x) - (2   x)))$ $\mapsto$ $((((((-(x) <= -(9)) || ((0 == (p - 2)) \&\& (1 >= (p - y)) \&\& ((x + y) <= -(6)) \&\& (0 >= (-(p) + y)))) || ((0 == (p - 2)) \&\& (x <= -(7)) \&\& (0 >= (p - y)))) || ((0 == (p - 1)) \&\& (0 >= (p - y)) \&\& ((x - y) <= -(9)) \&\& (2 >= (-(p) + y)) \&\& ((x + y) <= -(5)))) || ((0 == (p - 1)) \&\& (x <= -(7)) \&\& (0 >= (p - y)) \&\& ((x + y) <= -(2)))) || ((0 == (p - 1)) \&\& (1 >= (-(x) - y)) \&\& ((-(p) + x) <= -(8)))),(8 >= x)\&\&!(((0 == (p - 2)) \&\& (1 >= (p - y)) \&\& ((x + y) <= -(6)) \&\& (0 >= (-(p) + y))))\&\&!(((0 == (p - 2)) \&\& (x <= -(7)) \&\& (0 >= (p - y))))\&\&!(((0 == (p - 1)) \&\& (0 >= (p - y)) \&\& ((x - y) <= -(9)) \&\& (2 >= (-(p) + y)) \&\& ((x + y) <= -(5))))\&\&!(((0 == (p - 1)) \&\& (x <= -(7)) \&\& (0 >= (p - y)) \&\& ((x + y) <= -(2))))\&\&!(((0 == (p - 1)) \&\& (1 >= (-(x) - y)) \&\& ((-(p) + x) <= -(8))))$  \\
\bottomrule
