\ttt{afagp-T.c} & \rExact  & 160.3    & 1  & v,v & $\ell_{21}:!(((((((x   z) - x) - y) + 1) + c) < k))$ $\mapsto$ $(0 >= (-(c) + k)),((c - k) <= -(1))$  \\
\ttt{afefp-T.c} & \rExact  & 312.1    & 2  & v,en,v,v & $\ell_{23}:((((((((2   Y)   xp) - ((2   X)   y)) - X) + (2   Y)) - v) + c) <= k)$ $\mapsto$ $0 \geq c-k,k-c \leq -1$  \\
\ttt{agafp-T.c} & \rExact  & 24.4     & 1  & v,v & $\ell_{22}:(((((c + (4   x)) - (((y   y)   y)   y)) - (((2   y)   y)   y)) - (y   y)) < k)$ $\mapsto$ $((c - k) <= -(1)),(0 >= (-(c) + k))$  \\
\ttt{neg-afefp-F.c} & \rExact  & 233.2    & 1  & v,v & $\ell_{17}:(((((1 + (x   z)) - x) - (z   y)) + c) < k)$ $\mapsto$ $((c - k) <= -(1)),(0 >= (-(c) + k))$  \\
\ttt{neg-afp-F.c} & \rExact  & 68.2     & 2  & v,en,v,v & $\ell_{17}:(((((c + (6   x)) - (((2   y)   y)   y)) - ((3   y)   y)) - y) < k)$ $\mapsto$ $((c - k) <= -(1)),(((0 + (k   1)) + (c   -1)) <= 0)$  \\
\bottomrule
